

## Question 2:

a)

That is, every string derivable in  $G_1$  is derivable in  $G_2$  and vice-versa.

iff for every position  $n \geq 1$ , the  $n$ -th value produced by  $G_1$  equals the  $n$ -th value produced by  $G_2$ .

Formally, if we write

$$v_1(n) = G_1.\text{next}().\text{value},$$

$$v_2(n) = G_2.\text{next}().\text{value},$$

then

$$G_1 \equiv G_2 \Leftrightarrow \forall n \in \mathbb{N}^+, v_1(n) = v_2(n).$$

In other words, they yield the same infinite sequence of numbers.

c)

נוכיח באינדוקציה על איבר  $n$

בסיס:  $\text{Fib}_1$  הגדרנו ש  $\text{Fib}_1(1)=1$

$$\text{Fib}_2 \rightarrow \text{Fib}_2(1) = (((1+\sqrt{5})/2) - ((1-\sqrt{5})/2))/\sqrt{5} \Rightarrow \frac{2\sqrt{5}}{\sqrt{5}} = \frac{\sqrt{5}}{\sqrt{5}} = 1$$

אז  $\text{Fib}_1(1) = \text{Fib}_2(1)$

טענה: נניח כי עד מספר  $n$  מתקיים ש  $\text{Fib}_1(n) = \text{Fib}_2(n)$

צעד: נוכיח עבור  $n+1$

$$\begin{aligned} \text{Fib}_1(n+1) &= \text{Fib}_1(n) + \text{Fib}_1(n-1) = \text{Fib}_2(n) + \text{Fib}_2(n-1) \\ \text{Fib}_2(n+1) &= \frac{\phi^{n+1} - \psi^{n+1}}{\sqrt{5}} = \frac{\phi^n \phi - \psi^n \psi}{\sqrt{5}} \\ &= \text{Fib}_2(n) \cdot \phi + \text{Fib}_2(n-1) \cdot \phi^0 = \text{Fib}_1(n+1) \end{aligned}$$

### Question 3.b:

Proposition: For any lists `lst1` and `lst2` and a continuation procedure `cont`,  $(\text{append\$ } \text{lst1 } \text{lst2 } \text{cont}) = (\text{cont } (\text{append } \text{lst1 } \text{lst2}))$ .

Proof: By induction on the length of `lst1`

Base: For the case of a `lst1` of length 0 [the empty list], the value of  $(\text{append } \text{lst1 } \text{lst2})$  is `lst2`, and the value of  $(\text{append\$ } \text{lst1 } \text{lst2 } \text{cont})$  is  $(\text{cont } \text{lst2})$ , which implies  $(\text{append\$ } \text{lst1 } \text{lst2 } \text{cont}) = (\text{cont } (\text{append } \text{lst1 } \text{lst2}))$ .

Induction step: We assume the proposition holds for `lst1` of length  $n$ , and show the proposition holds for `lst1` of a length  $n+1$ .

- (a) According to the code, the value of  $(\text{append } \text{lst1 } \text{lst2})$  is  $(\text{cons } (\text{car } \text{lst1}) (\text{append } (\text{cdr } \text{lst1}) \text{lst2}))$ .
- (b) According to the code, the value of  $(\text{append\$ } \text{lst1 } \text{lst2 } \text{cont})$  is  $(\text{append\$ } (\text{cdr } \text{lst1}) \text{lst2 } \text{cont2})$ , where `cont2` is the continuation procedure defined in lines 6-7.

Since the first operand of  $(\text{append\$ } (\text{cdr } \text{lst1}) \text{lst2 } \text{cont2})$  is a list of length  $n$ , according to the induction assumption:  $(\text{cont2 } (\text{append } (\text{cdr } \text{lst1}) \text{lst2})) = (\text{append\$ } (\text{cdr } \text{lst1}) \text{lst2 } \text{cont2})$ .

- $\rightarrow (\text{cont } (\text{cons } (\text{car } \text{lst1}) (\text{append } (\text{cdr } \text{lst1}) \text{lst2}))) = (\text{append\$ } (\text{cdr } \text{lst1}) \text{lst2 } \text{cont2}) \quad ;;; \text{code of cont 2}$
- $\rightarrow (\text{cont } (\text{append } \text{lst1 } \text{lst2})) = (\text{append\$ } (\text{cdr } \text{lst1}) \text{lst2 } \text{cont2}) \quad ;;; (a)$
- $\rightarrow (\text{cont } (\text{append } \text{lst1 } \text{lst2})) = (\text{append\$ } \text{lst1 } \text{lst2 } \text{cont}) \quad ;;; (b)$

5.1)

a)

$$\{t(s(s), G, s(U), p, t(K), s), t(s(G), G, K, p, t(K), U)\} \text{ : מילוי של } \{ \}$$

= מילוי של תחתית

$$t(s(s), G, s(U), p, t(K), s) = t(s(G), G, K, p, t(K), U)$$

$$[s(s)=s(G), G=G, s(U)=K, p=p, t(K)=t(K), s=U] \text{ : מילוי של } \{ \}$$

$$\{ s = G \} \text{ : נכונה, } s(s)=s(G) \text{ : נכונה}$$

$$\{ s = G, s(U)=K \} \text{ : נכונה, } s(U)=K \text{ : נכונה}$$

$$\{ s = G, s(U)=K, s=U \} \text{ : נכונה, } s=U \text{ : נכונה}$$

$$K = s(U) = s(s) \text{ : נכונה}$$

$$S = \{ G = s, U = s, K = s(s) \} \text{ : נכונה}$$

$$b) [ [w|v] \mid [v|k] ] = [ [v|v] \mid w ]$$

$\{ \}$  : נכונה

$$\{ w = v \} \text{ : } [w|v] = [v|v] \text{ : נכונה}$$

$$[v|k] = v \text{ : נכונה, } [v|k] \text{ : נכונה}$$

5.3)  $\text{plus}(\text{succ}(\text{zero}), x, \text{succ}(\text{succ}(\text{zero})))$

$\%3 \{ x_1 = \text{succ}(\text{zero}) \}$  ↓  
 $x = \text{zero}$  ↓

$\text{plus}(\text{succ}(\text{succ}(\text{zero})), \text{zero}, \text{succ}(\text{succ}(\text{zero})))$   
 $\%2 \{ x_1 = \text{succ}(\text{succ}(\text{zero})) \}$  ↓  
 $\text{natural-number}(\text{succ}(\text{succ}(\text{zero})))$

$\%2 \{ x_1 = \text{succ}(\text{zero}) \}$  ↓  
 $\text{natural-number}(\text{succ}(\text{zero}))$

$\%1 \{ x_1 = \text{zero} \}$  ↓  
 $\text{natural-number}(\text{zero})$

הוכחה סיום,  $x = \text{zero}$

pr